playground/uart_model/clockScript.sml
@@ -1,0 +1,111 @@
+(********************************************)
+(*   properties of next and rel_sequances   *)
+(********************************************)
+
+open HolKernel Parse boolLib bossLib;
+open m0Theory progTheory m0_progTheory stateTheory m0_stepTheory;
+open boolSimps;
+val _ = new_theory "clock"
+
+(* next is strictly monotonically increasing in clock cycles *)
+		  
+val  NEXT_MONO = Q.store_thm("NEXT_MONO",
+
+`!s. s.count < (Next s).count`,
+    cheat
+
+(* also works thus far:  
+`!s. s.count <= (Next s).count`,
+*)
+);
+
+
+
+(*
+execution sequences are strictly monotonically increasing
+in clock cycles
+ *)
+val SEQ_MONO1 = Q.prove(
+`!s i seq. rel_sequence (NEXT_REL $= NextStateM0) seq s ==>  (seq i).count <= (seq (i+1)).count`,
+    SIMP_TAC (std_ss++LET_ss) [rel_sequence_def,NEXT_REL_def, PULL_EXISTS, PULL_FORALL, NextStateM0_def, DECIDE ``SUC i= i+1``]>>
+    REPEAT STRIP_TAC>>
+    Q.PAT_X_ASSUM `!n:num._` ( MP_TAC o (Q.SPEC `i:num`))>>
+    IF_CASES_TAC>>(
+        STRIP_TAC>>
+        Q.PAT_X_ASSUM `x:m0_state=_` (( SIMP_TAC std_ss) o (fn x => x::[]) o GSYM)
+    )>>
+    MP_TAC( SPEC ``(seq (i:num)):m0_state`` NEXT_MONO ) >>
+    DECIDE_TAC
+);
+
+val SEQ_MONO2 = Q.prove(
+`!s  i d seq. rel_sequence (NEXT_REL $= NextStateM0) seq s ==>  (seq i).count <= (seq (i+d)).count`,
+    REPEAT STRIP_TAC>>
+    Induct_on `d`>-(
+        SIMP_TAC arith_ss [] )>>
+    (MP_TAC o Q.SPECL [`s`, `i+d`, `seq`] ) SEQ_MONO1>>
+    FULL_SIMP_TAC arith_ss [DECIDE ``i + SUC d=i+ d+1``]
+);
+
+
+val SEQ_MONO_A = Q.store_thm("SEQ_MONO_A",
+`!s a b seq. rel_sequence (NEXT_REL $= NextStateM0) seq s /\  (seq a).count < (seq b).count ==> a <= b `,
+    REPEAT STRIP_TAC>>
+    Cases_on `a<=b`>>(
+	ASM_SIMP_TAC std_ss [])>>
+    MP_TAC (Q.SPECL [`s`, `b`, `a-b`, `seq`] SEQ_MONO2)>>
+    FULL_SIMP_TAC arith_ss []
+);
+
+val SEQ_MONO_B = Q.store_thm("SEQ_MONO_B",
+`!s a b seq. rel_sequence (NEXT_REL $= NextStateM0) seq s /\ a <= b ==> (seq a).count <= (seq b).count `,
+    REPEAT STRIP_TAC>>
+    MP_TAC (Q.SPECL [`s`, `a`, `b-a`, `seq`] SEQ_MONO2)>>
+    FULL_SIMP_TAC arith_ss []
+);
+
+val SEQ_UNIQUE1 = Q.prove(
+`!s i seq. rel_sequence (NEXT_REL $= NextStateM0) seq s /\ ( (seq i).count = (seq (i+1)).count)  ==>
+(seq i = seq (i+1))
+ `,
+    SIMP_TAC (std_ss++LET_ss) [
+         rel_sequence_def,NEXT_REL_def,
+         PULL_EXISTS, PULL_FORALL, 
+         NextStateM0_def, DECIDE ``SUC i= i+1``]>>
+    REPEAT STRIP_TAC>>
+    Q.PAT_X_ASSUM `!n:num._` ( MP_TAC o (Q.SPEC `i:num`))>>
+    IF_CASES_TAC>>(
+        STRIP_TAC>>
+        ASM_SIMP_TAC std_ss []
+    )>>
+        MP_TAC( SPEC ``(seq (i:num)):m0_state`` NEXT_MONO ) >>	
+        ASM_SIMP_TAC std_ss []
+);
+
+val SEQ_MONO2 = Q.prove(
+`!s  i d seq. rel_sequence (NEXT_REL $= NextStateM0) seq s /\ ( (seq i).count = (seq (i+d)).count) ==>( (seq i) = (seq (i+d)))`,
+    REPEAT STRIP_TAC>>
+    Induct_on `d`>-(
+        SIMP_TAC arith_ss [] )>>
+    (MP_TAC o Q.SPECL [`s`, `i`, `i+d`, `seq`] ) SEQ_MONO_B>>
+    (MP_TAC o Q.SPECL [`s`, `i+d`, `i+d+1`, `seq`] ) SEQ_MONO_B>>
+    (MP_TAC o Q.SPECL [`s`, `i+d`, `seq`] ) SEQ_UNIQUE1>>
+    FULL_SIMP_TAC arith_ss [DECIDE ``i + SUC d=(i+ d)+1``]
+);
+
+val SEQ_MONO = Q.store_thm("SEQ_UNIQUE",
+`!s a b seq. rel_sequence (NEXT_REL $= NextStateM0) seq s /\ ( (seq a).count = (seq b).count) ==> ((seq a) = (seq b)) `,
+    REPEAT STRIP_TAC>>
+    Cases_on `a=b`>>(
+	ASM_SIMP_TAC std_ss [])>>
+    Cases_on `a<b`>|[
+	MP_TAC (Q.SPECL [`s`, `a`, `b-a`, `seq`] SEQ_MONO2)>>
+	`a+(b-a)=b` by DECIDE_TAC>>
+	ASM_SIMP_TAC std_ss[],
+  
+	MP_TAC (Q.SPECL [`s`, `b`, `a-b`, `seq`] SEQ_MONO2)>>
+	`b+(a-b)=a` by DECIDE_TAC>>
+	ASM_SIMP_TAC std_ss[]
+    ]
+);
+val _ = export_theory();
