playground/uart_model/m0_NITScript.sml
@@ -1,0 +1,394 @@
+(*loadPath := ("/home/daniil/HOL/examples/l3-machine-code/m0/model"::(!loadPath));
+loadPath := ("/Home/daniil/HOL/examples/l3-machine-code/common"::(!loadPath));
+loadPath := ("/home/daniil/HOL/examples/l3-machine-code/m0/prog"::(!loadPath));
+loadPath := ("/home/daniil/HOL/examples/l3-machine-code/m0/decompiler"::(!loadPath));
+*)
+
+open HolKernel Parse boolLib bossLib;
+open stateTheory m0_stepTheory boolSimps;
+open wordsTheory;
+open m0Theory;
+open boolSimps;
+open optionTheory;
+open m0_progLib;
+open m0_progTheory;
+open progTheory;
+
+val _ = new_theory "m0_NIT";
+
+val mem_eq_def = Define`
+mem_eq region mem1 mem2 = 
+   (!x. x IN region ==> ((mem1 x) = (mem2 x)))
+`;
+
+val m0_r_eq_def = Define `
+m0_r_eq region s1 s2 = 
+   (mem_eq region s1.MEM s2.MEM)
+`;
+
+val m0_non_r_eq_def = Define `
+    m0_non_r_eq region s1 s2 = (
+	(s1.AIRCR = s2.AIRCR)/\
+	(s1.CCR = s2.CCR)/\
+	(s1.CONTROL = s2.CONTROL)/\
+	(s1.CurrentMode = s2.CurrentMode)/\
+	(s1.ExceptionActive = s2.ExceptionActive)/\
+	(s1.NVIC_IPR = s2.NVIC_IPR)/\
+	(s1.PRIMASK = s2.PRIMASK)/\
+	(s1.PSR = s2.PSR)/\
+	(s1.REG = s2.REG)/\
+	(s1.SHPR2 = s2.SHPR2)/\
+	(s1.SHPR3 = s2.SHPR3)/\
+	(s1.VTOR = s2.VTOR)/\
+	(s1.count = s2.count)/\
+	(s1.exception = s2.exception)/\
+	(s1.pcinc = s2.pcinc)/\
+	(s1.pending = s2.pending)/\
+	(mem_eq {x|  x NOTIN region } s1.MEM s2.MEM))`;
+
+(** There is no flow to a memory region from the rest of the state 
+    During the next tranisition
+
+    for arbitrary content of the region, the next instruciton does not change the content of the region
+**)
+val NIT_STEP_to_def = Define` 
+ NIT_STEP_to region s = (
+  !s'.  m0_non_r_eq region s s' ==> m0_r_eq region s' (Next s') 
+ )`;
+
+(** There is no information flow to the rest of the state from this region 
+    During the next tranisition 
+    
+    Swaping out the content of the region arbitraraly does not affect the execution of the rest of the state.
+**)
+val NIT_STEP_from_def = Define` 
+ NIT_STEP_from region s = (
+  !s'. m0_non_r_eq region s s'==> m0_non_r_eq region (Next s) (Next s') 
+)`;
+
+val NIT_STEP_def = Define`
+NIT_STEP region s = (NIT_STEP_from region s) /\ (NIT_STEP_to region s) 
+`;
+
+val NIT_STEP_thm = Q.store_thm ("NIT_STEP_thm",
+    `!region s. NIT_STEP region s =  
+         (!s'. m0_non_r_eq region s s'==> 
+            (m0_non_r_eq region (Next s) (Next s') /\
+             m0_r_eq region s' (Next s')))`,
+    SIMP_TAC std_ss [NIT_STEP_def, NIT_STEP_to_def, NIT_STEP_from_def]>>
+    METIS_TAC []
+);
+
+val NIT_W_def = Define`
+NIT region s t =   ! s' seq seq' i.   m0_non_r_eq region s s' /\ 
+               rel_sequence (NEXT_REL $= NextStateM0) seq  s /\
+               rel_sequence (NEXT_REL $= NextStateM0) seq' s' /\
+               m0_non_r_eq region s s' /\ ((seq i).count = t) ==>   
+                   m0_non_r_eq region (seq i) (seq' i) /\
+                   m0_r_eq region s' (seq' i)`;
+
+val NIT_def = Define`
+NIT region s t =   ! s' seq seq' i.   m0_non_r_eq region s s' /\ 
+               rel_sequence (NEXT_REL $= NextStateM0) seq  s /\
+               rel_sequence (NEXT_REL $= NextStateM0) seq' s' /\
+               m0_non_r_eq region s s' /\ ((seq i).count <= t) ==>   
+                   m0_non_r_eq region (seq i) (seq' i) /\
+                   m0_r_eq region s' (seq' i)`;
+
+(********************************)
+(*   uart eqvivalance thearems  *)
+(********************************)
+
+val mem_eq_refl_thm = Q.store_thm("mem_eq_refl_thm",
+    `!region mem1 mem2. 
+	(mem_eq region mem1 mem2)  = (mem_eq region mem2 mem1) `,
+	 METIS_TAC[mem_eq_def]
+);
+
+val mem_eq_trans_thm = Q.store_thm("mem_eq_trans_thm",
+    `!region mem1 mem2 mem3. 
+	(mem_eq region mem1 mem2) /\ 
+	(mem_eq region mem2 mem3) ==>
+	    (mem_eq region mem1 mem3) `,
+SIMP_TAC std_ss [mem_eq_def]);
+
+val m0_r_eq_refl_thm = Q.store_thm ("m0_r_eq_refl_thm",
+`!s1 s2 region. m0_r_eq region s1 s2 =  m0_r_eq region s2 s1`,
+SIMP_TAC std_ss [m0_r_eq_def, mem_eq_refl_thm]);
+
+val m0_non_r_eq_refl_thm = Q.store_thm ("m0_non_r_eq_refl_thm",
+`!s1 s2 region. m0_non_r_eq region s1 s2 =  m0_non_r_eq region s2 s1`,
+SIMP_TAC std_ss [m0_non_r_eq_def, mem_eq_refl_thm]>>
+METIS_TAC [mem_eq_refl_thm]
+);
+
+val m0_non_r_eq_trans_thm = Q.store_thm ("m0_non_r_eq_trans_thm",
+`!s1 s2 s3 region.
+    m0_non_r_eq region s1 s2 /\
+    m0_non_r_eq region s2 s3 ==>
+        m0_non_r_eq region s1 s3`,
+REPEAT GEN_TAC>>
+SIMP_TAC std_ss [m0_non_r_eq_def]>>
+METIS_TAC[ mem_eq_trans_thm]);
+
+val m0_r_eq_trans_thm = Q.store_thm ("m0_r_eq_trans_thm",
+`!s1 s2 s3 region.
+    m0_r_eq region s1 s2 /\
+    m0_r_eq region s2 s3 ==>
+        m0_r_eq region s1 s3`,
+REPEAT GEN_TAC>>
+SIMP_TAC std_ss [m0_r_eq_def]>>
+METIS_TAC[ mem_eq_trans_thm]);
+
+(*******************************************************)
+(*            NIT theorems                             *)
+(*******************************************************)
+
+
+val NIT_STEP_TRANS_thm = Q.store_thm("NIT_STEP_TRANS_thm",
+`!r s q . NIT_STEP r s ∧ m0_non_r_eq r q s ==> NIT_STEP r q`,
+SIMP_TAC std_ss [ NIT_STEP_thm]>>
+    METIS_TAC [m0_non_r_eq_trans_thm, m0_non_r_eq_refl_thm ]);
+
+val NIF_STEP_to_UNION_thm = Q.store_thm ("NIF_STEP_to_UNION_thm",
+    `! s region1 region2. NIT_STEP_to region1 s  /\ NIT_STEP_to region2 s ==> 
+                          NIT_STEP_to (region1 UNION region2) s`,
+    cheat
+    (*
+    the idea was to do a conterposition prof
+
+    SIMP_TAC std_ss [PULL_FORALL, NIT_STEP_def, NIT_STEP_to_def, NIT_STEP_from_def]>>
+	     REPEAT STRIP_TAC>>
+	     Q.PAT_X_ASSUM `!a b._` (MP_TAC o Q.SPECL [`s'`, `s'`])>>
+	     REPEAT STRIP_TAC
+	     
+    Cases_on `m0_r_eq (region1 ∪ region2) s' (Next s')`>>ASM_SIMP_TAC std_ss []
+
+    nagate the conscusions 
+    ` ~ m0_r_eq region1 s' (Next s')` by cheat
+    ` ~ m0_r_eq region2 s' (Next s')` by cheat
+    and get negation of assumptions
+
+    `~(m0_non_r_eq region1 s s')` by METIS_TAC []
+    `~(m0_non_r_eq region2 s s')` by METIS_TAC []
+
+    and then show the contradiction
+   REPEAT ( Q.PAT_X_ASSUM `_==>_` (fn x=> ALL_TAC))
+   REPEAT ( PAT_X_ASSUM ``~ m0_r_eq _ _ (Next s')`` (fn x=> ALL_TAC))
+   ( PAT_X_ASSUM ``_`` MP_TAC)
+   REWITE_TAC []
+
+   ONCE_SIMP_TAC (std_ss) [m0_non_r_eq_def]
+   
+   def_SIMP_TAC (std_ss++pred_setLib.PRED_SET_ss) [m0_non_r_eq_def, mem_eq_def, PULL_EXISTS, PULL_FORALL]
+   REPEAT STRIP_TAC
+   
+   PAT_ASSUM ``!x._`` (MP_TAC o (Q.SPEC `x'`))>>
+   PAT_ASSUM ``!x._`` (MP_TAC o (Q.SPEC `x`))
+   
+   *)
+);
+
+val NIF_STEP_from_UNION_thm = Q.store_thm ("NIF_STEP_from_UNION_thm",
+    `! s region1 region2. NIT_STEP_from region1 s  /\ NIT_STEP_from region2 s ==> 
+                          NIT_STEP_from (region1 UNION region2) s`,
+    cheat
+);
+
+val NIF_STEP_UNION_thm = Q.store_thm ("NIF_STEP_UNION_thm",
+    `! s region1 region2. NIT_STEP region1 s  /\ NIT_STEP region2 s ==> 
+                          NIT_STEP (region1 UNION region2) s`,
+    cheat
+);
+
+
+
+(*****************************)
+(*   Run & equance stuff     *)
+(*****************************)
+
+val M0_SEQUENCE_THM = prove(`` rel_sequence (NEXT_REL $= NextStateM0) seq s <=>
+  (seq 0 = s) ∧ !n. if (Next(seq n)).exception = NoException then seq (n+1) = Next (seq n) else seq (n+1) = seq n``,
+    SIMP_TAC (std_ss++boolSimps.LET_ss++boolSimps.COND_elim_ss) [
+	DECIDE ``SUC n = n + 1n``, rel_sequence_def, NEXT_REL_EQ, NextStateM0_def]>>
+    METIS_TAC[]);
+
+val RunM0_def = Define `(RunM0 s 0n = s) /\
+                         (RunM0 s k = let 
+                           s' = RunM0 s (k-1)
+                        in if (Next (s')).exception = NoException 
+                           then Next(s')
+                           else s')`;
+
+
+val RunM0_SEQUENCE_THM = prove(
+``! s seq.
+  (rel_sequence (NEXT_REL $= NextStateM0) seq s)  <=> (seq = (RunM0 s))``,
+    REPEAT STRIP_TAC>>
+    SIMP_TAC std_ss [M0_SEQUENCE_THM, FUN_EQ_THM, PULL_FORALL]>>
+    EQ_TAC>-(
+	SPEC_TAC (``s:m0_state``, ``s:m0_state``)>>
+	SIMP_TAC std_ss [ PULL_FORALL]>>
+	Induct_on `x`>-( 
+	    METIS_TAC[RunM0_def ]
+	) >>
+	REPEAT STRIP_TAC >>
+	ONCE_REWRITE_TAC [RunM0_def]>>
+	SIMP_TAC (arith_ss++LET_ss) [NextStateM0_def, optionTheory.option_CLAUSES] >>
+	Q.PAT_X_ASSUM `!s:m0_state._` (fn x=> MP_TAC (SPEC ``s:m0_state`` x))>>
+	ASM_SIMP_TAC std_ss[]>>
+	Q.PAT_X_ASSUM `!n._` (fn x=> MP_TAC (SPEC ``x:num`` x))>>
+	METIS_TAC[DECIDE ``SUC x= x+1``]
+    )>>
+    SIMP_TAC std_ss [ PULL_FORALL]>>
+    REPEAT STRIP_TAC >-  
+    (SIMP_TAC std_ss [RunM0_def])>>
+    IF_CASES_TAC>> ASM_SIMP_TAC (arith_ss++LET_ss) [RunM0_def, DECIDE ``n+1=SUC n``]
+);
+
+
+
+(* UART specific shite*)
+val uart_region_def = Define`
+(* TODO: change to bit masking? *)
+uart_region = {addr| addr >= 0x40002000w /\ addr <= 0x4000256Cw}
+`;
+(*
+
+val no_if_to_uart_def = Define`
+no_if_to_uart s = no_flow_to uart_region s`;
+
+
+val no_if_from_uart_def = Define`
+no_if_from_uart s = no_flow_from uart_region s`;
+
+
+val ward_region_def = Define`
+(* TODO: change to bit masking? *)
+ward_region x = {addr| (addr = x) \/ (addr = x+1w) \/
+                         (addr = x+2w) \/ (addr = x+3w)}
+`;
+
+val no_if_to_word_def = Define`
+no_if_to_word addr s = no_flow_to ward_region s`;
+
+
+val no_if_from_word_def = Define`
+no_if_from_word addr s = no_flow_from (ward_region addr) s`;
+=======
+val mem_region_eq_def = Define`
+mem_eq region mema memb = 
+   (!x. x IN region ==> ((mema x) = (memb x)))
+`
+
+val m0_region_eq_def = Define `
+m0_region_eq region s1 s2 = 
+   (mem_eq region s1.MEM s2.MEM)
+`
+DB.find "m0_state"
+val m0_non_region_eq_def = Define `
+  m0_non_uart_eq s1 s2 = (
+
+(s1.AIRCR = s2.AIRCR)/\
+(s1.CCR = s2.CCR)/\
+(s1.CONTROL = s2.CONTROL)/\
+(s1.CurrentMode = s2.CurrentMode)/\
+ExceptionActive
+NVIC_IPR
+PRIMASK
+PSR
+REG
+SHPR2
+SHPR3
+VTOR
+count
+exception
+pcinc
+pending
+
+   (a.REG = b.REG) /\ (a.count = b.count) /\ (non_uart_mem_eq a.MEM b.MEM)
+   (* Do we need to include other parts of the state ?, yes*)
+  )
+`;
+
+val m0_non_uart_eq_def = Define `
+  m0_non_uart_eq a b = (
+   (a.REG = b.REG) /\ (a.count = b.count) /\ (non_uart_mem_eq a.MEM b.MEM)
+   (* Do we need to include other parts of the state ?, yes*)
+  )
+`;
+
+val m0_uart_eq_def = Define `
+  m0_uart_eq a b = 
+    (uart_mem_eq a.MEM b.MEM)
+`;
+
+
+val no_if_uart_2_cpu_def = Define`
+no_if_uart_2_cpu s0 = (
+    ! s1. m0_non_uart_eq s0 s1 ==> m0_non_uart_eq (Next s0) (Next s1)
+)`;
+
+val no_if_cpu_2_uart_def = Define`
+no_if_uart_2_cpu s0 = (
+    (** we need to fex next instruction to be executed, if code is always located in a fixed region of memory then it would be better to constain that memory region instead **)
+    ! s1. (** s1.REG PC = s0.REG PC /\ s0.MEM (R s PC) = s1.MEM(R s' PC) **) => 
+         m0_uart_eq s0 s1 ==> m0_uart_eq (Next s0) (Next s1)
+)`;
+
+val no_if_2_cpu_no_load_thm = prove (`` !s.  no_if_uart_2_cpu s  ==> ~( load_uart_reg s)``,
+STRIP_TAC
+EQ_TAC
+SIMP_TAC std_ss [no_if_uart_2_cpu_def]
+Induct_on `s` 
+Induct_on `f1`
+);
+
+
+(** experements to investigate proving information flow for decompiled code **)
+val m0_non_addr_eq_def = Define `
+  m0_non_uart_eq addr a b = (
+   (a.REG = b.REG) /\ (a.count = b.count) /\ 
+          (!addr'. (addr' <> addr) ==> ((a.MEM addr')=(b.MEM addr')))
+   (* Do we need to include other parts of the state ?*)
+  )
+`;
+
+
+val m0_addr_eq_def = Define `
+  m0_addr_eq addr a b =
+       (** TODO: might need to fix PC, (s.MEM PC) and regesters used by the instruction at s.MEM PC **)
+    ((a.MEM addr)=(b.MEM addr))
+`;
+
+
+(** this version without ext.quant. **)
+val mem_written_1_def = Define`
+    mem_written_1 s a = let
+      s'  = s with MEM updated_by (\m. (a =+ 0w) m );  
+      s'' = s with MEM updated_by (\m. (a =+ ~0w) m)
+    in ~((((Next(s')).MEM a) = 0w) /\ ( ((Next(s'')).MEM a)=~0w)) 
+`;
+
+(** this version is more in Information flow style**)
+
+
+val nif_from_addr_def = Define`
+    nif_from_addr a s = !s'. (** TODO: 
+                if next operation is fixed!!! ==> **) 
+         m0_addr_eq a s s' ==>
+             m0_addr_eq a (Next s) (Next s')           
+`;
+
+val nif_to_addr_def = Define`
+    nif_to_addr a s = !s'. (** TODO: 
+                if next operation is fixed!!! ==> **) 
+         m0_non_addr_eq a s s' ==>
+             m0_non_addr_eq a (Next s) (Next s')           
+`;
+
+val if_to_addr_def = Define`
+    if_to_addr_def a s = ?s'. (m0_non_addr_eq a s s' ) /\ ~(m0_non_addr_eq a (Next s) (Next s'))
+`;
+*)
+val _ = export_theory();
